src/reflection/FStar.Reflection.Interpreter.fs
@@ -44,8 +44,8 @@ let reflection_primops : list<N.primitive_step> =
 
         mk1 "__inspect_bv" inspect_bv unembed_binder embed_string;
         mk2 "__compare_binder" order_binder unembed_binder unembed_binder embed_order;
-
         mk1 "__type_of_binder" (fun (b,q) -> b.sort) unembed_binder embed_term;
+        mk2 "__is_free" is_free unembed_binder unembed_term embed_bool;
 
         mk2 "__term_eq" FStar.Syntax.Util.term_eq unembed_term unembed_term embed_bool;
 
